coq/coq/Target.v
@@ -5,6 +5,13 @@ Require Import Arith Lia.
 Require Import Infrastructure.
 
 
+Lemma eqIndTypTarget_refl : forall T,
+    eqIndTypTarget T T.
+Proof.
+Admitted.
+
+#[local] Hint Resolve eqIndTypTarget_refl : core.
+
 Lemma wf_rcd_lookup : forall i T Ti,
   wf_typ T ->
   Tlookup i T = Some Ti ->
@@ -14,7 +21,7 @@ Proof.
   gen i Ti.
   induction WF; intros; simpl in LK; inverts LK.
   case_if*.
-  - inverts* H2.
+  - inverts* H3.
 Qed.
 
 Lemma rcd_typ_concat : forall T1 T2 T3,
@@ -56,6 +63,7 @@ Proof.
     unfolds. case_if*.
 Qed.
 
+
 Lemma wf_rcd_concat : forall T1 T2 T3,
     wf_typ T1 -> wf_typ T2 ->
     rec_typ T1 -> rec_typ T2 ->
@@ -80,21 +88,73 @@ Lemma target_typing_wf_1 : forall E t A,
 Proof with eauto; destruct_uniq; solve_uniq.
   introv H.
   induction* H.
-  - pick_fresh x. forwards*: H1 x...
+  - pick_fresh x. forwards*: H0 x...
   - pick_fresh x. forwards*: H0 x...
 Qed.
 
-Lemma target_typing_wf_2 : forall G t T,
-   target_typing G t T -> wf_typ T.
+
+Lemma context_wf_inv_1 : forall E G,
+    wf_ctx (E ++ G) -> wf_ctx E.
+Proof.
+  introv HW. gen G. induction* E; intros.
+  - simpl in HW. inverts* HW.
+Qed.
+
+Lemma context_wf_inv_2 : forall E G,
+    wf_ctx (E ++ G) -> wf_ctx G.
+Proof.
+  introv HW. gen G. induction* E; intros.
+  - simpl in HW. inverts* HW.
+Qed.
+
+Lemma context_wf_compose : forall E F,
+    wf_ctx E -> wf_ctx F -> wf_ctx (E ++ F).
+Proof with eauto using context_wf_inv_1, context_wf_inv_2.
+  introv HW1 HW2.
+  gen F. induction E; intros; simpl...
+  inverts* HW1.
+Qed.
+
+Lemma target_typing_wf_2 : forall E t A,
+    target_typing E t A -> wf_ctx E.
+Proof with eauto using context_wf_inv_1, context_wf_inv_2.
+  introv H.
+  induction* H.
+  all: instantiate_cofinites...
+  all: inverts* H0.
+Qed.
+
+Lemma target_context_binds_wf : forall x At Gt,
+    binds x At Gt -> wf_ctx Gt -> wf_typ At.
+Proof.
+  introv HB HW.
+  induction Gt.
+  - exfalso. applys* binds_nil_iff.
+  - inverts* HB; inverts* HW.
+    Unshelve. applys ttyp.
+    all: eauto.
+Qed.
+
+Lemma wf_typ_look_up_wf : forall l At Bt,
+    Tlookup l At = Some Bt -> wf_typ At -> wf_typ Bt.
 Proof with eauto.
+  introv Heq WF. gen l Bt.
+  induction WF; intros; try solve_by_invert.
+  inverts Heq. case_if*.
+  - inverts* H3.
+Qed.
+
+Lemma target_typing_wf_typ : forall G t T,
+    target_typing G t T -> wf_typ T.
+Proof with eauto using target_typing_wf_2, target_context_binds_wf.
   intros Ga t T Htyp.
-  induction Htyp...
-  all: pick fresh x...
-  - (* T_App *)
-    inversion IHHtyp1...
-  - (* T_Proj *)
-    eapply wf_rcd_lookup...
-  - applys* wf_rcd_concat At Bt Ct.
+  induction* Htyp.
+  - applys target_context_binds_wf; tassumption.
+  - instantiate_cofinites...
+  - instantiate_cofinites...
+  - inverts* IHHtyp1.
+  - eauto using wf_typ_look_up_wf.
+  - applys* wf_rcd_concat H1.
 Qed.
 
 Lemma target_typing_lc_texp : forall G t T,
@@ -109,10 +169,10 @@ Qed.
 
 
 Lemma lookup_field_in_value : forall v T i Ti,
-  value v ->
-  target_typing [] v T ->
-  Tlookup i T = Some Ti ->
-  exists ti, tlookup i v = Some ti /\ target_typing [] ti Ti.
+    value v ->
+    target_typing [] v T ->
+    Tlookup i T = Some Ti ->
+    exists ti, tlookup i v = Some ti /\ target_typing [] ti Ti.
 Proof with try solve_by_invert.
   introv Val Typ LK.
   induction Typ; try solve_by_invert.
@@ -123,10 +183,9 @@ Proof with try solve_by_invert.
 Qed.
 
 
-
 Theorem progress : forall t T,
-     target_typing [] t T ->
-     value t \/ exists t', t >-> t'.
+    target_typing [] t T ->
+    value t \/ exists t', t >-> t'.
 Proof with try solve_by_invert.
   introv Typ.
   inductions Typ...
@@ -158,17 +217,27 @@ Proof with try solve_by_invert.
     all: right; exists; eauto using target_typing_lc_texp.
 Qed.
 
+Lemma context_wf_compose_middle : forall E F G,
+    wf_ctx (E ++ G) -> wf_ctx F -> wf_ctx (E ++ F ++ G).
+Proof.
+  introv WF1 WF2.
+  lets: context_wf_inv_1 WF1.
+  lets: context_wf_inv_2 WF1.
+  eauto using context_wf_compose.
+Qed.
+
 Lemma target_weakening : forall G E F t T,
     target_typing (E ++ G) t T ->
+    wf_ctx F ->
     uniq (E ++ F ++ G) ->
     target_typing (E ++ F ++ G) t T.
-Proof.
-  introv Typ; gen F;
-    inductions Typ; introv Ok; autos*.
+Proof with eauto using context_wf_compose_middle.
+  introv Typ WF HU; gen F;
+    inductions Typ; intros; autos...
     + (* abs *)
       pick fresh x and apply TTyping_Abs; eauto.
       rewrite_env (([(x, At)] ++ E) ++ F ++ G).
-      apply~ H1.
+      apply~ H0.
       solve_uniq.
     + (* fix *)
       pick fresh x and apply TTyping_Fix.
@@ -179,7 +248,7 @@ Qed.
 
 Lemma target_weakening_simpl : forall E F e T,
     target_typing E e T ->
-    uniq (F ++ E) ->
+    uniq (F ++ E) -> wf_ctx F ->
     target_typing (F ++ E) e T.
 Proof.
   intros.
@@ -187,49 +256,124 @@ Proof.
   applys* target_weakening.
 Qed.
 
-
 Lemma target_weakening_empty : forall G t T,
-    uniq G -> target_typing [] t T -> target_typing G t T.
+    uniq G -> wf_ctx G -> target_typing [] t T -> target_typing G t T.
 Proof.
-  introv Uni Typ.
+  introv Uni Wf Typ.
   rewrite_env ([]++G++[]).
   applys* target_weakening.
 Qed.
-
 
 
 Lemma substitution_preserves_typing : forall (E F : tctx) t u S T (z : atom),
     target_typing (F ++ [(z,S)] ++ E) t T ->
     target_typing E u S ->
     target_typing (F ++ E) ([z ~>> u] t) T.
-Proof with eauto.
+Proof with eauto using context_wf_inv_1, context_wf_inv_2.
   introv Typ1 Typ2.
-  inductions Typ1.
+  lets T1: Typ1. inductions T1.
+  all: assert (wf_ctx (F ++ E)) by
+    ( lets HW: target_typing_wf_2 Typ1;
+      lets W1: context_wf_inv_1 HW; lets W2: context_wf_inv_2 HW;
+      lets W3: context_wf_inv_2 W2; applys* context_wf_compose ).
   all: simpl...
   - (* var *)
     simpl. case_if; subst.
     + forwards* : binds_mid_eq H1.
-      subst. applys* target_weakening_simpl.
-    + forwards* : binds_remove_mid H1.
+      subst. applys* target_weakening_simpl...
+    + forwards* : binds_remove_mid H1...
   - (* abs *)
     pick fresh x and apply TTyping_Abs...
+    rewrite subst_texp_open_texp_wrt_texp_var...
+    forwards*: H0 x.
+    rewrite_env (((x, At) :: F) ++ [(z, S)] ++ E)...
+    rewrite_env (((x, At) :: F) ++ [(z, S)] ++ E)...
+    eauto.
+  - (* fixpoint *)
+    pick fresh x and apply TTyping_Fix...
     rewrite_env (((x, At) :: F) ++ E).
     rewrite subst_texp_open_texp_wrt_texp_var...
-    applys* H1.
-    eauto.
+Qed.
+
+
+Lemma subst_var_typing : forall x A G t B y,
+    target_typing ((x, A) :: G) (open_texp_wrt_texp t (texp_var_f x)) B ->
+    x `notin` fv_texp t -> y `notin` (dom G `union` fv_texp t) ->
+    target_typing ((y, A) :: G) (open_texp_wrt_texp t (texp_var_f y)) B.
+Proof.
+  introv HT HNx HNy.
+  destruct (x == y); subst*.
+  forwards HU: target_typing_wf_1 HT.
+  rewrite (@subst_texp_intro x); eauto.
+  rewrite_env ( [] ++ ( (y, A) :: G) ).
+  applys* substitution_preserves_typing A.
+  - rewrite_env ( [(x, A)] ++ [(y, A)] ++ G ).
+    applys* target_weakening.
+    + constructor*. lets HW: target_typing_wf_2 HT. applys* target_context_binds_wf HW.
+    + destruct_uniq. solve_uniq.
+  - constructor*; inverts* HU.
+    lets HW: target_typing_wf_2 HT. inverts* HW.
+Qed.
+
+
+Lemma substitution_preserves_typing_relax : forall E F t u S S' T z,
+    target_typing (F ++ [(z,S)] ++ E) t T ->
+    target_typing E u S' -> eqIndTypTarget S S' ->
+    exists T', eqIndTypTarget T T' /\ target_typing (F ++ E) ([z ~>> u] t) T'.
+Proof with eauto using context_wf_inv_1, context_wf_inv_2.
+  introv Typ1 Typ2 Eq.
+  lets T1: Typ1. inductions T1.
+  all: assert (wf_ctx (F ++ E)) by
+    ( lets HW: target_typing_wf_2 Typ1;
+      lets W1: context_wf_inv_1 HW; lets W2: context_wf_inv_2 HW;
+      lets W3: context_wf_inv_2 W2; applys* context_wf_compose ).
+  all: simpl...
+  - (* var *)
+    simpl. case_if; subst.
+    + forwards* : binds_mid_eq H1.
+      subst. exists S'. split*. applys* target_weakening_simpl...
+    + forwards* : binds_remove_mid H1.
+  - (* abs *)
+    pick fresh x. instantiate_cofinites...
+    rewrite_env (((x, At) :: F) ++ [(z, S)] ++ E) in H...
+    forwards* (T' & ? & HT): H0 H.
+    exists (ttyp_arrow At T'). split*.
+    pick fresh y and apply TTyping_Abs.
+    rewrite_env ((x, At) :: F ++ E) in HT.
+    rewrite <- subst_texp_open_texp_wrt_texp_var in HT...
+    forwards* : subst_var_typing HT.
+    applys* subst_texp_fresh_mutual; solve_notin.
+    applys notin_union_3. solve_notin.
+    applys* subst_texp_fresh_mutual; solve_notin.
+  - Abort.
+
   - (* fixpoint *)
     pick fresh x and apply TTyping_Fix...
     rewrite_env (((x, At) :: F) ++ E).
     rewrite subst_texp_open_texp_wrt_texp_var...
     applys* H0.
     eauto.
+
+
+    exists. split.
+    eapply (Typ_abs (union L (singleton z))); eauto.
+    intros.
+    forwards~(?&?&?): H0 x.
+    rewrite_env (([(x, A)] ++ F) ++ [(z, S)] ++ E).
+    reflexivity.
+    (* lc_e_abs_exists *)
+    rewrite subst_exp_open_exp_wrt_exp_var; auto.
+    rewrite_env (([(x, A)] ++ F) ++ E).
+    apply subsub2sub in H3.
+    forwards*: Typing_chk_sub H2 H3.
+    auto.
 Qed.
 
 
 Theorem preservation : forall t t' T,
     target_typing [] t T ->
     t >-> t' ->
-    target_typing [] t' T.
+    exists T', eqIndTypTarget T T' /\ target_typing [] t' T'.
 Proof with eauto using rcd_typ_concat.
   introv Typ Red. gen t'.
   inductions Typ; intros;
@@ -259,10 +403,11 @@ Proof with eauto using rcd_typ_concat.
     inverts* Red.
     + inverts Typ1. inverts~ H1.
     + inverts Typ1. inverts~ H1.
-      destruct H10.
+      destruct H9.
       * applys* TTyping_RcdCons...
         forwards*: lookup_concat_typ. left. rewrite* H2.
       * applys* TTyping_RcdCons...
         forwards*: lookup_concat_typ_none.
-        destruct H14 as [Heq|Heq]; rewrite <- Heq; eauto.
+        rewrite H2.
+        destruct H15 as [Heq|Heq]; rewrite Heq; eauto.
 Qed.
